PAC: starting missing initialisation

PAC/PAC_Polynoms_Term.thy
@@ -78,6 +78,10 @@ definition term_poly_list_rel :: \<open>(term_poly_list \<times> term_poly) set\
      distinct xs \<and>
      sorted_wrt (rel2p var_order_rel) xs}\<close>
 
+definition unsorted_term_poly_list_rel :: \<open>(term_poly_list \<times> term_poly) set\<close> where
+  \<open>unsorted_term_poly_list_rel = {(xs, ys).
+     ys = mset xs}\<close>
+
 definition poly_list_rel :: \<open>_ \<Rightarrow> (('a \<times> int) list \<times> mset_polynom) set\<close> where
   \<open>poly_list_rel R = {(xs, ys).
      (xs, ys) \<in> \<langle>R \<times>\<^sub>r int_rel\<rangle>list_rel O list_mset_rel \<and>
@@ -119,6 +123,14 @@ lemma sorted_poly_list_rel_empty_l[simp]:
   \<open>([], s') \<in> sorted_poly_list_rel_wrt S T \<longleftrightarrow> s' = {#}\<close>
   by (cases s')
     (auto simp: sorted_poly_list_rel_wrt_def list_mset_rel_def br_def)
+
+
+definition fully_unsorted_poly_list_rel :: \<open>_ \<Rightarrow> (('a \<times> int) list \<times> mset_polynom) set\<close> where
+  \<open>fully_unsorted_poly_list_rel R = {(xs, ys).
+     (xs, ys) \<in> \<langle>R \<times>\<^sub>r int_rel\<rangle>list_rel O list_mset_rel}\<close>
+ 
+abbreviation fully_unsorted_poly_rel where
+  \<open>fully_unsorted_poly_rel \<equiv> fully_unsorted_poly_list_rel unsorted_term_poly_list_rel\<close>
 
 
 end
